commit

Projects/Esolangs/Lang_001/Basic.lean
@@ -10,46 +10,46 @@ def exprId : Expr :=
 def progId : Prog where
   defs := [⟨1, exprId⟩]
 
-def exprSelf (i : ℕ) : Expr :=
-  call (.custom i) [.arg 0]
+def exprLoop (i : ℕ) : Expr :=
+  .call (.custom i) [.arg 0]
 
-def progSelf : Prog where
-  defs := [⟨1, exprSelf 0⟩]
+def progLoop : Prog where
+  defs := [⟨1, exprLoop 0⟩]
 
 def refZero : Expr :=
-  call (.custom 1) []
+  .call (.custom 1) []
 
 def refOne : Expr :=
-  call (.custom 2) []
+  .call (.custom 2) []
 
 def exprZero : Expr :=
-  call (.builtin .sub) [refZero, refZero]
+  .call (.builtin .sub) [refZero, refZero]
 
 def exprOne : Expr :=
-  call (.builtin .succ) [refZero]
+  .call (.builtin .succ) [refZero]
 
 def exprNot : Expr :=
-  call (.builtin .sub) [refOne, .arg 0]
+  .call (.builtin .sub) [refOne, .arg 0]
 
 def exprBool : Expr :=
-  call (.custom 3) [call (.custom 3) [.arg 0]]
+  .call (.custom 3) [.call (.custom 3) [.arg 0]]
 
 def exprAdd : Expr :=
-  call (.builtin .sub)
-    [ call (.builtin .sub)
-      [ call (.builtin .sub)
-        [ call (.builtin .succ) [call (.builtin .succ) [
-            call (.custom 5)
-              [ call (.builtin .sub) [.arg 0, refOne]
-              , call (.builtin .sub) [.arg 1, refOne]
-              ]
-          ]]
-        , call (.custom 3) [.arg 0]
-        ]
-      , call (.custom 3) [.arg 1]
+  .call (.builtin .sub)
+  [ .call (.builtin .sub)
+    [ .call (.builtin .sub)
+      [ .call (.builtin .succ) [.call (.builtin .succ) [
+          .call (.custom 5)
+            [ .call (.builtin .sub) [.arg 0, refOne]
+            , .call (.builtin .sub) [.arg 1, refOne]
+            ]
+        ]]
+      , .call (.custom 3) [.arg 0]
       ]
-    , call (.custom 5) [refZero, refZero]
+    , .call (.custom 3) [.arg 1]
     ]
+  , .call (.custom 5) [refZero, refZero]
+  ]
 
 def exprMain₁ : Expr :=
   exprId
@@ -61,7 +61,7 @@ def prog₁ : Prog where
     ⟨0, exprOne⟩,
     ⟨1, exprNot⟩,
     ⟨1, exprBool⟩,
-    -- ⟨2, exprAdd⟩,
+    ⟨2, exprAdd⟩,
   ]
 
 def prog₁FS : List (List ℕ → ℕ) :=
@@ -70,7 +70,7 @@ def prog₁FS : List (List ℕ → ℕ) :=
   , fn 0 λ _ => 1
   , fn 1 λ xs => if xs[0]! = 0 then 1 else 0
   , fn 1 λ xs => if xs[0]! = 0 then 0 else 1
-  -- , fn 2 λ xs => xs[0]! + xs[1]!
+  , fn 2 λ xs => xs[0]! + xs[1]!
   ]
 
 -- #check 0 #exit
@@ -79,11 +79,15 @@ def prog₁FS : List (List ℕ → ℕ) :=
 
 @[simp] theorem defs_progId : progId.defs = [⟨1, exprId⟩] := rfl
 @[simp] theorem main_progId : progId.main = ⟨1, exprId⟩ := rfl
-@[simp] theorem wf_exprId : exprId.WF progId 1 := by simp [Expr.WF, exprId]
+@[simp] theorem wf_exprId {prog} : exprId.WF prog 1 := by simp [Expr.WF, exprId]
 @[simp] theorem wf_defId : (Def.mk 1 (.arg 0)).WF progId := wf_exprId
 @[simp] theorem arity_zero_progId : progId.arity 0 = 1 := rfl
 @[simp] theorem expr_zero_progId : progId.expr 0 = exprId := rfl
-@[simp] theorem Expr.run_arg {i prog f args} : (arg i).eval prog f args = args[i]! := rfl
+
+@[simp]
+theorem Expr.run_arg {i prog f args} : (arg i).eval prog f args = args[i]! := by
+  simp [eval]
+
 @[simp] theorem Prog.defs_mk {ds} : defs ⟨ds⟩ = ds := rfl
 @[simp] theorem Builtin.arity_succ : Builtin.succ.arity = 1 := rfl
 @[simp] theorem Builtin.arity_sub : Builtin.sub.arity = 2 := rfl
@@ -92,7 +96,10 @@ def prog₁FS : List (List ℕ → ℕ) :=
 @[simp] theorem Target.f_custom {fs i} : (custom i).f fs = fs[i]! := rfl
 @[simp] theorem Target.arity_custom {prog i} : (custom i).arity prog = prog.arity i := rfl
 @[simp] theorem Prog.main_mk {defs} : main ⟨defs⟩ = defs[0]! := rfl
-@[simp] theorem Expr.wf_arg {prog n i} : (arg i).WF prog n ↔ i < n := by rfl
+
+@[simp]
+theorem Expr.wf_arg {prog n i} : (arg i).WF prog n ↔ i < n := by
+  simp [WF]
 
 @[simp, instance]
 theorem wf_progId : progId.WF := by
@@ -104,15 +111,12 @@ theorem wf_progId : progId.WF := by
   obtain ⟨f, rfl⟩ := h₁; simp at h₂ h₃ ⊢; grind
 
 @[simp]
-theorem Expr.run_call' {prog fs args t xs} : (Expr.call' t xs).eval prog fs args =
-t.f fs (List.range (t.arity prog) |>.map λ i => xs i |>.eval prog fs args) := rfl
+theorem Expr.run_call {prog fs args t xs} : (Expr.call t xs).eval prog fs args =
+t.f fs (xs.map λ x => x.eval prog fs args) := by
+  simp [eval]
 
-@[simp]
-theorem Expr.run_call {prog fs args t xs} : (call t xs).eval prog fs args =
-t.f fs (List.range (t.arity prog) |>.map λ i => xs[i]! |>.eval prog fs args) := rfl
-
-theorem not_wf_progSelf : ¬progSelf.WF := by
-  unfold progSelf exprSelf
+theorem not_wf_progLoop : ¬progLoop.WF := by
+  unfold progLoop exprLoop
   rintro ⟨-, -, -, h⟩; contrapose! h; clear h
   rw [not_exiu_iff_or]; right
   use [fn 1 λ _ => 0], [fn 1 λ _ => 1]; unfold fn
@@ -124,13 +128,17 @@ theorem Prog.compatible_fs {prog : Prog} [H : prog.WF] : prog.Compatible prog.fs
   Classical.epsilon_spec # H.exiu_compatible.exists
 
 @[simp]
+theorem eval_exprId {prog fs xs} : exprId.eval prog fs xs = xs[0]! := by
+  simp [exprId]
+
+@[simp]
 theorem run_progId {n} : progId.run n = n := by
   simp [Prog.run, Prog.eval]; have h := @progId.compatible_fs.eval_eq
-  simp at h; specialize @h [n]; simp at h; exact h
+  simp at h; specialize @h [n]; simpa using h
 
 @[simp]
 theorem wf_expr_prog₁_main₁ : exprMain₁.WF prog₁ 1 := by
-  constructor
+  simp [exprMain₁]
 
 @[simp]
 theorem wf_def_prog₁_main₁ : Def.WF prog₁ ⟨1, exprMain₁⟩ := by
@@ -149,12 +157,9 @@ prog.HasTarget (.custom i) ↔ i < prog.defs.length := by rfl
 @[simp] theorem Builtin.f_sub : f .sub = (λ xs => xs[0]! - xs[1]!) := rfl
 
 @[simp]
-theorem Expr.wf_call' {prog t args n} : (call' t args).WF prog n ↔ prog.HasTarget t ∧
-∀ ⦃j⦄, if t.arity prog ≤ j then args j = default else args j |>.WF prog n := by rfl
-
-@[simp]
 theorem Expr.wf_call {prog t args n} : (call t args).WF prog n ↔ prog.HasTarget t ∧
-∀ ⦃j⦄, if t.arity prog ≤ j then args[j]! = default else args[j]! |>.WF prog n := by rfl
+args.length = t.arity prog ∧ ∀ e ∈ args, e.WF prog n := by
+  simp [WF]
 
 theorem Prog.fs_eq_of_compatible {prog : Prog} {fs} [hp : prog.WF]
 (h : prog.Compatible fs) : prog.fs = fs :=
@@ -168,48 +173,65 @@ instance {prog : Prog} {t} : Decidable # prog.HasTarget t := by
 
 -- #check 0 #exit
 
------
+theorem exprAdd_aux {f : ℕ → ℕ → ℕ} (h : ∀ x y, f x y = f (x - 1) (y - 1) + 2 -
+(if x = 0 then 1 else 0) - (if y = 0 then 1 else 0) - f 0 0) : f = (· + ·) := by
+  ext x y
+  have h₁ : f 0 0 = 0
+  · specialize h 0 0
+    simpa using h
+  induction x generalizing y
+  · specialize h 0
+    simp at h
+    induction y
+    · specialize h 0
+      simpa using h
+    nm y ih
+    specialize h (y + 1)
+    simp_all
+  nm x ih
+  specialize h (x + 1) y
+  simp_all
+  specialize ih (y + 1)
+  grind
 
-@[simp] theorem length_defs_prog₁ : prog₁.defs.length = 5 := rfl
+-- #check 0 #exit
+
+@[simp] theorem length_defs_prog₁ : prog₁.defs.length = 6 := rfl
 
 @[simp] theorem prog₁_arity_0 : prog₁.arity 0 = 1:= rfl
 @[simp] theorem prog₁_arity_1 : prog₁.arity 1 = 0:= rfl
 @[simp] theorem prog₁_arity_2 : prog₁.arity 2 = 0:= rfl
 @[simp] theorem prog₁_arity_3 : prog₁.arity 3 = 1:= rfl
 @[simp] theorem prog₁_arity_4 : prog₁.arity 4 = 1:= rfl
--- @[simp] theorem prog₁_arity_5 : prog₁.arity 5 = 2:= rfl
+@[simp] theorem prog₁_arity_5 : prog₁.arity 5 = 2:= rfl
 
 @[simp]
 theorem wf_prog₁_refZero {n} : refZero.WF prog₁ n := by
-  constructor <;> simp [prog₁]
+  simp [refZero]
 
 @[simp]
 theorem wf_expr_prog₁_exprZero {n} : exprZero.WF prog₁ n := by
-  constructor <;> simp; intro i; split_ifs with h; grind; simp at h
-  rw [show [_, _] = .replicate 2 _ by rfl]
-  rw [List.getElem!_eq_getElem h, List.getElem_replicate]; simp
+  simp [exprZero]
 
 @[simp]
 theorem wf_prog₁_refOne {n} : refOne.WF prog₁ n := by
-  constructor <;> simp [prog₁]
+  simp [refOne]
 
 @[simp]
 theorem wf_expr_prog₁_exprOne {n} : exprOne.WF prog₁ n := by
-  constructor <;> simp; intro i; split_ifs with h; grind; simp at h; simp [h]
+  simp [exprOne]
 
 @[simp]
 theorem wf_expr_prog₁_exprNot {n} : exprNot.WF prog₁ n ↔ 1 ≤ n := by
-  simp [exprNot]; constructor; contrapose!; simp; rintro rfl; use 1; simp
-  intro h i; split_ifs with h₁; grind
-  obtain rfl | rfl : i = 0 ∨ i = 1 := by omega
-  all_goals simp <;> omega
+  simp [exprNot]; omega
 
 @[simp]
 theorem wf_expr_prog₁_exprBool {n} : exprBool.WF prog₁ n ↔ 1 ≤ n := by
-  simp [exprBool]; constructor
-  · contrapose!; simp; rintro rfl; use 0; simp; use 0; simp
-  · intro h i; split_ifs with h₁; grind; simp at h₁; simp [h₁]
-    intro j; split_ifs with h₂; grind; simp at h₂; simp [h₂]; omega
+  simp [exprBool]; omega
+
+@[simp]
+theorem wf_expr_prog₁_exprAdd {n} : exprAdd.WF prog₁ n ↔ 2 ≤ n := by
+  simp [exprAdd]; omega
 
 -- #check 0 #exit
 
@@ -218,8 +240,8 @@ theorem compatible_prog₁_prog₁FS : prog₁.Compatible prog₁FS := by
   unfold prog₁FS; constructor <;> simp
   all_goals
     intro i h xs h₁
-    obtain rfl | rfl | rfl | rfl | rfl :
-      i = 0 ∨ i = 1 ∨ i = 2 ∨ i = 3 ∨ i = 4 := by omega
+    obtain rfl | rfl | rfl | rfl | rfl | rfl :
+      i = 0 ∨ i = 1 ∨ i = 2 ∨ i = 3 ∨ i = 4 ∨ i = 5 := by omega
   iterate 6 simp at h₁; simp [fn] <;> try grind
   all_goals nth_rw 1 [prog₁]; (try simp at h₁); simp [fn, h₁]
   · simp [exprMain₁, exprId]
@@ -227,12 +249,10 @@ theorem compatible_prog₁_prog₁FS : prog₁.Compatible prog₁FS := by
   · simp [exprOne, refZero, fn]
   · simp [exprNot, refOne, fn]; grind
   · simp [exprBool, fn]; grind
-  -- · simp [exprAdd, fn]; rw! [xs.eq_getElem_of_length_eq_two h₁]
-  --   simp; generalize xs[0] = x; generalize xs[1] = y; clear h₁ xs
-  --   simp [refOne, refZero, fn]; cases x; cases y <;> rfl; nm x
-  --   simp; cases y; rfl; nm y; simp; omega
-
--- #check 0 #exit
+  · simp [exprAdd, fn]; rw! [xs.eq_getElem_of_length_eq_two h₁]
+    simp; generalize xs[0] = x; generalize xs[1] = y; clear h₁ xs
+    simp [refOne, refZero, fn]; cases x; cases y <;> rfl; nm x
+    simp; cases y; rfl; nm y; simp; omega
 
 @[simp, instance]
 theorem wf_prog₁ : prog₁.WF := by
@@ -248,11 +268,22 @@ theorem wf_prog₁ : prog₁.WF := by
   have h_not : ∀ ⦃x⦄, fs[3]! [x] = if x = 0 then 1 else 0
   · intro x; specialize @h₃ 3 (by omega) [x] (by simp)
     simp [prog₁, exprNot, refOne] at h₃; grind
+  have h_bool : ∀ ⦃x⦄, fs[4]! [x] = if x = 0 then 0 else 1
+  · intro x; specialize @h₃ 4 (by omega) [x] (by simp)
+    simp [prog₁, exprBool] at h₃; grind
+  have h_add : ∀ ⦃x y⦄, fs[5]! [x, y] = x + y
+  · intro x y; specialize @h₃ 5 (by omega)
+    simp [prog₁, exprAdd, refOne, refZero] at h₃
+    simp [h_zero, h_one, h_not] at h₃
+    replace h₃ : ∀ x y, fs[5]! [x, y] = fs[5]! [x - 1, y - 1] + 2 -
+      (if x = 0 then 1 else 0) - (if y = 0 then 1 else 0) - fs[5]! [0, 0]
+    · intro x y; specialize @h₃ [x, y]; simp at h₃; omega
+    have h₄ := exprAdd_aux (f := λ x y => fs[5]! [x, y]) (by grind); grind
   rw [List.ext_getElem!_iff]; simp [h₁]; intro i h₄; ext xs
   specialize @h₂ i (by omega); specialize @h₃ i (by omega)
   specialize @h₂ xs; specialize @h₃ xs
-  obtain rfl | rfl | rfl | rfl | rfl :
-    i = 0 ∨ i = 1 ∨ i = 2 ∨ i = 3 ∨ i = 4 := by omega
+  obtain rfl | rfl | rfl | rfl | rfl | rfl :
+    i = 0 ∨ i = 1 ∨ i = 2 ∨ i = 3 ∨ i = 4 ∨ i = 5 := by omega
   all_goals simp [prog₁, fn] at h₂ h₃ ⊢
   · split_ifs with H
     · specialize h₃ H; simp [exprMain₁, exprId] at h₃; grind
@@ -261,12 +292,15 @@ theorem wf_prog₁ : prog₁.WF := by
   · simp [exprOne] at h₂ h₃; grind
   · simp [exprNot, refOne] at h₂ h₃; grind
   · simp [exprBool] at h₂ h₃; grind
-
--- #check 0 #exit
+  · simp [exprAdd, refOne, refZero] at h₂ h₃; grind
 
 @[simp]
 theorem fs_prog₁ : prog₁.fs = prog₁FS :=
   Prog.fs_eq_of_compatible compatible_prog₁_prog₁FS
+
+@[simp]
+theorem eval_prog₁ {i xs} : prog₁.eval i xs = prog₁FS[i]! xs := by
+  simp [Prog.eval]
 
 @[simp]
 theorem run_prog₁ {x} : prog₁.run x = x := by
