Projects/IndParser/Basic.lean
@@ -2,134 +2,134 @@ import Projects.IndParser.Defs
 
 namespace IndParser
 
-instance : ParType Parser := .par
-
-instance {α : Type*} {β : α → Type} [h : IsEmpty α] (x : α) : ParType (β x) :=
-  IsEmpty.false x |>.elim
-
-def botSpec : IndSpec where
-  tn := 0
-  cn := 1
-  ts := nofun
-  ctns := λ _ => 0
-  cts := nofun
-  cs := λ bot _ => (.up [bot.down], nofun)
-
-def bot : Parser :=
-  botSpec.toParser.down
-
-def εSpec : IndSpec where
-  tn := 0
-  cn := 1
-  ts := nofun
-  ctns := λ _ => 1
-  cts := λ _ _ => Parser
-  cs := λ _ _ => (λ x => .up [x, x.concat x], nofun)
-
-def ε : Parser :=
-  εSpec.toParser.down
-
--- #check 0 #exit
-
------
-
-@[simp]
-theorem mkFinFn_zero.{u, v} {α : Fin 0 → Type u} {β : Type v}
-{f : (∀ n, α n) → β} : mkFinFn f = .up (f nofun) := rfl
-
-@[simp]
-theorem mkFinFn_succ.{u, v} {n} {α : Fin (n + 1) → Type u} {β : Type v}
-{f : (∀ n, α n) → β} : mkFinFn f = λ (x : α 0) => @mkFinFn n
-(λ ⟨k, h⟩ => α ⟨k + 1, by omega⟩) β (λ ps₁ => f # λ ⟨k, hk⟩ =>
-match k with | 0 => x | k + 1 => ps₁ ⟨k, by omega⟩) := by
-  funext x; congr; ext ps; dsimp; congr; ext k
-  rcases k with ⟨⟨⟩ | _, hk⟩ <;> rfl
-
-@[simp]
-theorem callFinFn_mkFinFn.{u, v} {n : ℕ} {α : Fin n → Type u} {β : Type v}
-{f : (∀ n, α n) → β} {ps : ∀ n, α n} : callFinFn (mkFinFn f) ps = f ps := by
-  induction n
-  · dsimp [callFinFn, mkFinFn]
-    congr; ext n; rcases n with ⟨n, h⟩; simp at h
-  nm n ih; simp [callFinFn]
-  specialize @ih (λ ⟨k, h⟩ => α ⟨k + 1, by omega⟩) _ _
-  · exact λ ps₁ => f λ ⟨k, hk⟩ => match k with
-    | 0 => ps 0
-    | k + 1 => ps₁ ⟨k, by omega⟩
-  · exact λ ⟨k, hk⟩ => ps ⟨k + 1, by omega⟩
-  convert ih using 2; ext k; rcases k with ⟨⟨⟩ | _, h⟩ <;> rfl
-
-@[simp]
-theorem callFinFn_zero.{u, v} {α : Fin 0 → Type u} {β : Type v} {ps} {r : β} :
-callFinFn (α := α) ⟨r⟩ ps = r := rfl
-
-@[simp]
-theorem finFn_zero.{u, v} {α : Fin 0 → Type u} {β : Type v} :
-FinFn α β = ULift.{max u v + 1} β := rfl
-
-@[simp] theorem Word.xs_eps : eps.xs = [] := rfl
-@[simp] theorem Word.xs_concat {a b : Word} : (a.concat b).xs = a.xs ++ b.xs := rfl
-@[simp] theorem Parser.words_bot : Parser.bot.words = ∅ := rfl
-@[simp] theorem Parser.words_eps : Parser.eps.words = {.eps} := rfl
-@[simp] theorem Parser.words_univ : Parser.univ.words = .univ := rfl
-@[simp] theorem Parser.words_inter {a b : Parser} : (a.inter b).words = a.words ∩ b.words := rfl
-
-@[simp]
-theorem Parser.words_concat {a b : Parser} : (a.concat b).words =
-{w | ∃ w₁ ∈ a.words, ∃ w₂ ∈ b.words, w₁.concat w₂ = w} := rfl
-
-@[simp]
-theorem Word.eps_concat {a : Word} : eps.concat a = a := by
-  ext; simp
-
-@[simp]
-theorem Word.concat_eps {a : Word} : a.concat eps = a := by
-  ext; simp
-
-@[simp]
-theorem Parser.eps_concat {a : Parser} : eps.concat a = a := by
-  ext; simp
-
-@[simp]
-theorem Parser.concat_eps {a : Parser} : a.concat eps = a := by
-  ext; simp
-
--- #check 0 #exit
-
------
-
-@[simp]
-theorem bot_eq : bot = .bot := by
-  ext x : 2
-  simp [bot, IndSpec.toParser]
-  intro h
-  apply @IndSpec.Ind.rec botSpec (motive := λ _ _ _ => False)
-  on_goal 2 => exact h
-  rintro n ps xs ys part ind w h₁ h₂ rfl rfl h₃ ih
-  simp [botSpec] at ind
-  rcases ind with ⟨⟨ind⟩⟩
-  simp [botSpec] at h₃
-  simp at h₂
-  subst h₂
-  simp at h₃
-  exact ih _ w h₃
-
+-- instance : ParType Parser := .par
+-- 
+-- instance {α : Type*} {β : α → Type} [h : IsEmpty α] (x : α) : ParType (β x) :=
+--   IsEmpty.false x |>.elim
+-- 
+-- def botSpec : IndSpec where
+--   tn := 0
+--   cn := 1
+--   ts := nofun
+--   ctns := λ _ => 0
+--   cts := nofun
+--   cs := λ bot _ => (.up [bot.down], nofun)
+-- 
+-- def bot : Parser :=
+--   botSpec.toParser.down
+-- 
+-- def εSpec : IndSpec where
+--   tn := 0
+--   cn := 1
+--   ts := nofun
+--   ctns := λ _ => 1
+--   cts := λ _ _ => Parser
+--   cs := λ _ _ => (λ x => .up [x, x.concat x], nofun)
+-- 
+-- def ε : Parser :=
+--   εSpec.toParser.down
+-- 
+-- -- #check 0 #exit
+-- 
+-- -----
+-- 
 -- @[simp]
--- theorem ε_eq : ε = .eps := by
+-- theorem mkFinFn_zero.{u, v} {α : Fin 0 → Type u} {β : Type v}
+-- {f : (∀ n, α n) → β} : mkFinFn f = .up (f nofun) := rfl
+-- 
+-- @[simp]
+-- theorem mkFinFn_succ.{u, v} {n} {α : Fin (n + 1) → Type u} {β : Type v}
+-- {f : (∀ n, α n) → β} : mkFinFn f = λ (x : α 0) => @mkFinFn n
+-- (λ ⟨k, h⟩ => α ⟨k + 1, by omega⟩) β (λ ps₁ => f # λ ⟨k, hk⟩ =>
+-- match k with | 0 => x | k + 1 => ps₁ ⟨k, by omega⟩) := by
+--   funext x; congr; ext ps; dsimp; congr; ext k
+--   rcases k with ⟨⟨⟩ | _, hk⟩ <;> rfl
+-- 
+-- @[simp]
+-- theorem callFinFn_mkFinFn.{u, v} {n : ℕ} {α : Fin n → Type u} {β : Type v}
+-- {f : (∀ n, α n) → β} {ps : ∀ n, α n} : callFinFn (mkFinFn f) ps = f ps := by
+--   induction n
+--   · dsimp [callFinFn, mkFinFn]
+--     congr; ext n; rcases n with ⟨n, h⟩; simp at h
+--   nm n ih; simp [callFinFn]
+--   specialize @ih (λ ⟨k, h⟩ => α ⟨k + 1, by omega⟩) _ _
+--   · exact λ ps₁ => f λ ⟨k, hk⟩ => match k with
+--     | 0 => ps 0
+--     | k + 1 => ps₁ ⟨k, by omega⟩
+--   · exact λ ⟨k, hk⟩ => ps ⟨k + 1, by omega⟩
+--   convert ih using 2; ext k; rcases k with ⟨⟨⟩ | _, h⟩ <;> rfl
+-- 
+-- @[simp]
+-- theorem callFinFn_zero.{u, v} {α : Fin 0 → Type u} {β : Type v} {ps} {r : β} :
+-- callFinFn (α := α) ⟨r⟩ ps = r := rfl
+-- 
+-- @[simp]
+-- theorem finFn_zero.{u, v} {α : Fin 0 → Type u} {β : Type v} :
+-- FinFn α β = ULift.{max u v + 1} β := rfl
+-- 
+-- @[simp] theorem Word.xs_eps : eps.xs = [] := rfl
+-- @[simp] theorem Word.xs_concat {a b : Word} : (a.concat b).xs = a.xs ++ b.xs := rfl
+-- @[simp] theorem Parser.words_bot : Parser.bot.words = ∅ := rfl
+-- @[simp] theorem Parser.words_eps : Parser.eps.words = {.eps} := rfl
+-- @[simp] theorem Parser.words_univ : Parser.univ.words = .univ := rfl
+-- @[simp] theorem Parser.words_inter {a b : Parser} : (a.inter b).words = a.words ∩ b.words := rfl
+-- 
+-- @[simp]
+-- theorem Parser.words_concat {a b : Parser} : (a.concat b).words =
+-- {w | ∃ w₁ ∈ a.words, ∃ w₂ ∈ b.words, w₁.concat w₂ = w} := rfl
+-- 
+-- @[simp]
+-- theorem Word.eps_concat {a : Word} : eps.concat a = a := by
+--   ext; simp
+-- 
+-- @[simp]
+-- theorem Word.concat_eps {a : Word} : a.concat eps = a := by
+--   ext; simp
+-- 
+-- @[simp]
+-- theorem Parser.eps_concat {a : Parser} : eps.concat a = a := by
+--   ext; simp
+-- 
+-- @[simp]
+-- theorem Parser.concat_eps {a : Parser} : a.concat eps = a := by
+--   ext; simp
+-- 
+-- -- #check 0 #exit
+-- 
+-- -----
+-- 
+-- @[simp]
+-- theorem bot_eq : bot = .bot := by
 --   ext x : 2
---   simp [ε, IndSpec.toParser]
---   symm; constructor
---   ·
---     rintro rfl
---     have h := @IndSpec.Ind.mk εSpec
---     simp only [εSpec, finFn_zero, Fin.forall_fin_zero_pi, mkFinFn_zero, ULift.forall,
---       ULift.up.injEq, forall_const] at h
---     specialize h (λ _ => .eps) [.eps, .eps] (λ _ _ => False) .bot .eps
---     simp only [IsEmpty.forall_iff, implies_true, Set.setOf_false, List.foldr_cons,
---       List.foldr_nil, Parser.words_inter, Parser.words_eps, Parser.words_univ,
---       Set.inter_univ, Set.inter_self, Set.mem_singleton_iff, forall_const] at h
---     specialize h rfl
---     simp only [callFinFn, Parser.concat_eps, forall_const] at h
---     specialize h (funext # by simp)
---     convert h
---   sorry
+--   simp [bot, IndSpec.toParser]
+--   intro h
+--   apply @IndSpec.Ind.rec botSpec (motive := λ _ _ _ => False)
+--   on_goal 2 => exact h
+--   rintro n ps xs ys part ind w h₁ h₂ rfl rfl h₃ ih
+--   simp [botSpec] at ind
+--   rcases ind with ⟨⟨ind⟩⟩
+--   simp [botSpec] at h₃
+--   simp at h₂
+--   subst h₂
+--   simp at h₃
+--   exact ih _ w h₃
+-- 
+-- -- @[simp]
+-- -- theorem ε_eq : ε = .eps := by
+-- --   ext x : 2
+-- --   simp [ε, IndSpec.toParser]
+-- --   symm; constructor
+-- --   ·
+-- --     rintro rfl
+-- --     have h := @IndSpec.Ind.mk εSpec
+-- --     simp only [εSpec, finFn_zero, Fin.forall_fin_zero_pi, mkFinFn_zero, ULift.forall,
+-- --       ULift.up.injEq, forall_const] at h
+-- --     specialize h (λ _ => .eps) [.eps, .eps] (λ _ _ => False) .bot .eps
+-- --     simp only [IsEmpty.forall_iff, implies_true, Set.setOf_false, List.foldr_cons,
+-- --       List.foldr_nil, Parser.words_inter, Parser.words_eps, Parser.words_univ,
+-- --       Set.inter_univ, Set.inter_self, Set.mem_singleton_iff, forall_const] at h
+-- --     specialize h rfl
+-- --     simp only [callFinFn, Parser.concat_eps, forall_const] at h
+-- --     specialize h (funext # by simp)
+-- --     convert h
+-- --   sorry
